Let us say that the index $i \in \{2, \ldots, n\}$ is an \emph{inversion point} for $\mathbf{p}$ and $\mathbf{q}$ if either
\[
\sum_{l=1}^{i} p_l < \sum_{l=1}^{i} q_l \quad \text{and} \quad \sum_{l=1}^{i-1} p_l > \sum_{l=1}^{i-1} q_l
\]
or, vice versa, if
\[
\sum_{l=1}^{i} p_l > \sum_{l=1}^{i} q_l \quad \text{and} \quad \sum_{l=1}^{i-1} p_l < \sum_{l=1}^{i-1} q_l.
\]

Let $2 \leq i_1 < i_2 < \cdots < i_k \leq n$ be all and the only inversion points for $\mathbf{p}$ and $\mathbf{q}$. Moreover, let
\[
\mathbf{t} = (t_1, \ldots, t_n) = \mathbf{p} \wedge \mathbf{q}
\]
and
\[
\mathbf{s} = (s_1, \ldots, s_n) = \beta(\mathbf{p}, \mathbf{q}).
\]

The proof of the theorem will be an immediate consequence of the following two claims, where we assume $i_0 = 0$ and $i_{k+1} = n + 1$ for the sake of definiteness. Hereafter, we shall use the common assumption that $0 \log \frac{1}{0} = 0$.

\textbf{Claim 1:} For each inversion point $i_r$, $r = 0, \ldots, k$, we have
\[
\sum_{l=i_r+1}^{i_{r+1}-1} p_l \log \frac{1}{p_l} + q_l \log \frac{1}{q_l} = \sum_{l=i_r+1}^{i_{r+1}-1} t_l \log \frac{1}{t_l}.
\]

\emph{Proof of Claim 1:} Indeed, let us assume, without loss of generality, that
\[
\sum_{l=1}^{i_r} p_l > \sum_{l=1}^{i_r} q_l.
\]

Then
\[
\sum_{l=1}^{i_r} s_l = \sum_{l=1}^{i_r} p_l
\]

and for all $s = i_r + 1, \ldots, i_{r+1} - 1$, we also have
\[
s_s = \sum_{l=1}^{s} p_l - \sum_{l=1}^{s} q_l = p_s.
\]

Accordingly, we have
\[
\sum_{l=1}^{i_r} t_l = \sum_{l=1}^{i_r} q_l
\]

and for all $s = i_r + 1, \ldots, i_{r+1} - 1$, we have
\[
t_s = \sum_{l=0}^{s} q_l - \sum_{l=0}^{s} t_l = q_s,
\]

which proves Claim 1.

As an immediate consequence of Claim 1, we have
\[
\sum_{l=i_r+1}^{i_{r+1}-1} \left( p_l \log \frac{1}{p_l} + q_l \log \frac{1}{q_l} - t_l \log \frac{1}{t_l} \right) = 0.
\]

\textbf{Claim 2:} For each inversion point $i_r$, $r = 1, 2, \ldots, k$, we have
\[
s_{i_r} \log \frac{1}{s_{i_r}} + t_{i_r} \log \frac{1}{t_{i_r}} > p_{i_r} \log \frac{1}{p_{i_r}} + q_{i_r} \log \frac{1}{q_{i_r}},
\]
where $p_{i_r}, q_{i_r}, s_{i_r}, t_{i_r} > 0$.

\emph{Proof of Claim 2:} Let us write $p, q, s, t$ instead of $p_{i_r}, q_{i_r}, s_{i_r}, t_{i_r}$, respectively. Without loss of generality let us assume that for the inversion point $i_r$ it holds that
\[
\sum_{l=1}^{i_r} p_l > \sum_{l=1}^{i_r} q_l \quad \text{and} \quad \sum_{l=1}^{i_r-1} p_l < \sum_{l=1}^{i_r-1} q_l.
\]

It follows that $s > p$ and $q > t$, so $s > t$. Moreover, it is not hard to see that $s + t = p + q$. Let $s = q + \Delta$, then $t = p - \Delta$ and $s + t = p + q$.

Then we have
\begin{align*}
s \log \frac{1}{s} + t \log \frac{1}{t} - p \log \frac{1}{p} - q \log \frac{1}{q}
&= - (s \log s + t \log t) + p \log p + q \log q \\
&= - (q + \Delta) \log (q + \Delta) - (p - \Delta) \log (p - \Delta) + p \log p + q \log q \\
&= (q \log q + p \log p) - \left( (q + \Delta) \log (q + \Delta) + (p - \Delta) \log (p - \Delta) \right) \\
&\geq (q + p + \Delta) \log \left( \frac{(q + p + \Delta)^2}{(q + \Delta)(p - \Delta)} \right) \quad \text{(by Jensen's inequality)} \\
&= (q + p + \Delta) \log \left( \frac{s + t + \Delta}{s + \Delta} \cdot \frac{s + t + \Delta}{t - \Delta} \right) \\
&= (q + p + \Delta) \log \left( \frac{(s + t + \Delta)^2}{(s + \Delta)(t - \Delta)} \right) > 0,
\end{align*}
since $s > t$ and $\Delta < t$.

The remaining case $s \leq t$ is completely symmetric, provided that we set $s = p + \Delta$ and $t = q - \Delta$. This concludes the proof of the Claim 2.

We are now ready to prove (12). We have
\begin{align*}
H(s) + H(t) - H(p) - H(q)
&= \sum_{l=1}^{k} \left( s_l \log \frac{1}{s_l} + t_l \log \frac{1}{t_l} - p_l \log \frac{1}{p_l} - q_l \log \frac{1}{q_l} \right) \\
&= \sum_{r=1}^{k} \left( \sum_{l=i_r+1}^{i_{r+1}-1} \left( s_l \log \frac{1}{s_l} + t_l \log \frac{1}{t_l} \right)
+ s_{i_r} \log \frac{1}{s_{i_r}} + t_{i_r} \log \frac{1}{t_{i_r}} \right. \\
&\quad \left. - p_{i_r} \log \frac{1}{p_{i_r}} - q_{i_r} \log \frac{1}{q_{i_r}} 
- \sum_{l=i_r+1}^{i_{r+1}-1} \left( p_l \log \frac{1}{p_l} + q_l \log \frac{1}{q_l} \right) \right) \\
&\quad + \sum_{l=1}^{i_1 - 1} \left( s_l \log \frac{1}{s_l} + t_l \log \frac{1}{t_l} 
- p_l \log \frac{1}{p_l} - q_l \log \frac{1}{q_l} \right) \\
&\quad + \sum_{l=i_k+1}^{n} \left( s_l \log \frac{1}{s_l} + t_l \log \frac{1}{t_l} 
- p_l \log \frac{1}{p_l} - q_l \log \frac{1}{q_l} \right) \\
&= \sum_{r=1}^{k} \left( s_{i_r} \log \frac{1}{s_{i_r}} + t_{i_r} \log \frac{1}{t_{i_r}} 
- p_{i_r} \log \frac{1}{p_{i_r}} - q_{i_r} \log \frac{1}{q_{i_r}} \right) 
\quad \text{(by Claim 1)} \\
&> 0 \quad \text{(by Claim 2).} \qedhere
\end{align*}